WIP in axioms

plugin/plugin_utils.mli
@@ -3,8 +3,8 @@ val string_of_chars : char list -> string
 
 val chars_of_string : string -> char list
 
-val extract_constant : Names.GlobRef.t -> string -> (BasicAst.kername * char list) * Datatypes.nat
+val extract_constant : Names.GlobRef.t -> string -> (((BasicAst.kername * char list) * Datatypes.nat) * int)
 
-val debug_mappings : (BasicAst.kername * string) list -> unit
+val debug_mappings : (((BasicAst.kername * char list) * Datatypes.nat) * int) -> unit
 
 val help_msg : string
